not working :(

backends/lean/Aeneas/Tactic/Step/InferPost.lean
@@ -14,8 +14,8 @@ open Lean Elab Meta Tactic TacticM
 
     `eliminate` controls which free variables to try clearing from the context before collecting
     escaping variables -/
-def inferPost (goal : MVarId) (eliminate : LocalDecl → Bool := fun _ => true) :
-    TacticM MVarId := withTraceNode `Step (fun _ => do pure m!"inferPost") <| withMainContext do
+def inferPost (goal : MVarId) (_eliminate : LocalDecl → Bool := fun _ => true) :
+    TacticM MVarId := withTraceNode `Step (fun _ => do pure m!"inferPost") <| goal.withContext do
   traceGoalWithNode "metavariable context"
   let goalTy ← instantiateMVars (← goal.getType)
 
@@ -32,8 +32,7 @@ def inferPost (goal : MVarId) (eliminate : LocalDecl → Bool := fun _ => true) 
   let mvarLCtx := (← postMVarId.getDecl).lctx
 
   -- Collect free vars not in the mvar's context or marked for elimination
-  let escapingLocalDecls := lclDecls.filter fun decl =>
-    mvarLCtx.contains decl.fvarId
+  let escapingLocalDecls := lclDecls.filter fun decl => !mvarLCtx.contains decl.fvarId
 
   -- Build postcondition: fun x₁ ... xₙ => ∃ vars..., x₁ = a₁ ∧ ... ∧ xₙ = aₙ ∧ props
   let argTys ← liftMetaM (args.mapM inferType)
