tests/lean/HigherOrder.lean
@@ -13,19 +13,10 @@ theorem applyF_spec (f : U32 → Result U32) (x : U32)
     applyF f x ⦃ post ⦄ := by
   simp [applyF]; exact hf
 
-/- set_option trace.Step true -/
-
-/--
-info: Try this:
-
-  [apply]     let* ⟨ y, y_post ⟩ ← [ +inferPost ] applyF_spec
-    case hf => let* ⟨ ⟩ ← [ +inferPost ] U32.add_spec
-    agrind
--/
-#guard_msgs in
+set_option trace.Step true in
 example (a : U32) (h : a.val + 1 ≤ U32.max) :
     applyF (fun x => x + 1#u32) a ⦃ y => y.val = a.val + 1 ⦄ := by
-  step*? +inferPost
+  step +inferPost
 
 -- Higher-order in 2 functions, operates on a pair of inputs/outputs
 def callPair (f : U32 → Result U32) (g : U32 → Result U32) (xy : U32 × U32) : Result (U32 × U32) := do
@@ -46,18 +37,18 @@ theorem callPair_spec (f g : U32 → Result U32) (xy : U32 × U32)
   simp [WP.spec, WP.theta, WP.wp_return]
   exact ⟨ha, hb⟩
 
-/--
-info: Try this:
-
-  [apply]     let* ⟨ ab, ab_post1, ab_post2 ⟩ ← [ +inferPost ] callPair_spec
-    case hf => let* ⟨ ⟩ ← [ +inferPost ] U32.add_spec
-    case hg => let* ⟨ ⟩ ← [ +inferPost ] U32.add_spec
-    agrind
--/
-#guard_msgs in
+/- /-- -/
+/- info: Try this: -/
+/--/
+/-   [apply]     let* ⟨ ab, ab_post1, ab_post2 ⟩ ← [ +inferPost ] callPair_spec -/
+/-     case hf => let* ⟨ ⟩ ← [ +inferPost ] U32.add_spec -/
+/-     case hg => let* ⟨ ⟩ ← [ +inferPost ] U32.add_spec -/
+/-     agrind -/
+/- -/ -/
+/- #guard_msgs in -/
 example (x y : U32) (hx : x.val + 1 ≤ U32.max) (hy : y.val + 2 ≤ U32.max) :
     callPair (fun a => a + 1#u32) (fun b => b + 2#u32) (x, y) ⦃ ab => ab.1.val = x.val + 1 ∧ ab.2.val = y.val + 2 ⦄ := by
-  step*? +inferPost
+  step* +inferPost
 
 -- Calls f then g in sequence
 def callFThenG (f g : U32 → Result U32) (x : U32) : Result U32 := do
